commit

src/mink/main.lean
@@ -1,39 +1,74 @@
 import tactic
 import tactic.induction
+import logic.function.iterate
 
 noncomputable theory
 open_locale classical
 
 inductive Expr : Type
-| M : Expr
 | K : Expr
 | S : Expr
+| M : Expr
 | App : Expr → Expr → Expr
 open Expr
 
 infixl ` ~ `:100 := App
 
-inductive Reduce : Expr → Expr → Prop
-| MK : Reduce (M ~ K) K
-| MS : Reduce (M ~ S) S
-| K {a b} : Reduce (K ~ a ~ b) a
-| S {a b c} : Reduce (S ~ a ~ b ~ c) (a ~ c ~ (b ~ c))
-| left {a b c} : Reduce a b → Reduce (a ~ c) (b ~ c)
-| right {a b c} : Reduce a b → Reduce (c ~ a) (c ~ b)
-| refl {a} : Reduce a a
-| trans {a b c} : Reduce a b → Reduce b c → Reduce a c
+def reduce : Expr → Expr
+| (K ~ a ~ b) := a
+| (S ~ a ~ b ~ c) := a ~ c ~ (b ~ c)
+| (M ~ K) := K
+| (M ~ S) := S
+| (M ~ a) := M ~ reduce a
+| a := a
 
-infix ` ==> `:50 := Reduce
+def R (e₁ e₂ : Expr) : Prop :=
+∃ (n : ℕ), e₂ = (reduce^[n]) e₁
+
+infix ` ==> `:50 := R
 
 -----
 
 @[refl]
-lemma Reduce.refl' {a} : a ==> a :=
-Reduce.refl
+lemma R.refl {a} : a ==> a :=
+by use [0, rfl]
 
 @[trans]
-lemma Reduce.trans' {a b c} (h₁ : a ==> b) (h₂ : b ==> c) : a ==> c :=
-Reduce.trans h₁ h₂
+lemma R.trans' {a b c} (h₁ : a ==> b) (h₂ : b ==> c) : a ==> c :=
+begin
+  cases h₁ with n₁ h₁, cases h₂ with n₂ h₂, use n₂ + n₁,
+  rw function.iterate_add_apply, substs h₁ h₂,
+end
+
+lemma not_R_iff {a b} : ¬a ==> b ↔ ∀ n, b ≠ (reduce^[n]) a :=
+by simp [R]
 
 -----
 
+lemma R_iff_of_reduce_eq_self_iff {a b}
+  (h : reduce a = a) : a ==> b ↔ a = b :=
+begin
+  split; intro h₁,
+  { contrapose h₁, rw [not_R_iff], intro n, induction n with n ih,
+    { tauto },
+    { simp [h, ih] } },
+  { subst h₁ },
+end
+
+-----
+
+def I := S ~ K ~ K
+
+lemma I_id {a} : I ~ a ==> a :=
+by use [2, rfl]
+
+-----
+
+-- lemma not_reduces_of {α : Sort*} (f : α → Expr) {a b : Expr} {z : α}
+--   (h₁ : f z = a)
+--   (h₂ : ∀ (x : α), f x ≠ b → ???)
+--   :
+--   a /=> b :=
+-- begin
+--   sorry
+-- end
